@prefix cito: <http://purl.org/spar/cito/> .
@prefix dc: <http://purl.org/dc/elements/1.1/> .
@prefix dct: <http://purl.org/dc/terms/> .  
@prefix foaf: <http://xmlns.com/foaf/0.1/> .
@prefix frbr: <http://purl.org/vocab/frbr/core#> .
@prefix owl: <http://www.w3.org/2002/07/owl#> .
@prefix prov: <http://www.w3.org/ns/prov#> .
@prefix rdfs: <http://www.w3.org/2000/01/rdf-schema#> .
@prefix rdf: <http://www.w3.org/1999/02/22-rdf-syntax-ns#> .
@prefix skos: <http://www.w3.org/2004/02/skos/core#> .
@prefix vann: <http://purl.org/vocab/vann/> .
@prefix xsd: <http://www.w3.org/2001/XMLSchema#> .
@prefix hico: <http://purl.org/emmedi/hico/> .

<http://purl.org/emmedi/hico/> a skos:ConceptScheme, owl:Ontology ;
    dc:title "The Historical Context Ontology (HiCO)"@en ;
    skos:prefLabel "The Historical Context Ontology (HiCO)"@en ;
    dc:contributor "Francesca Tomasi"@en, "Silvio Peroni"@en ;
    dc:creator "Marilena Daquino"@en ;
    dct:created "2019-10-02"^^xsd:date ;
    dct:issued "2020-03-31"^^xsd:date ;
    dct:modified "2020-03-31"^^xsd:date ;
    dc:description """The Historical Context Ontology (HiCO) is an OWL 2 DL ontology developed for representing the context of a claim. In particular, it addresses features characterising hermeneutical activities performed by scholars while generating new information (i.e. an interpretation act). It allows to represent and reason on reliability of argumentations around attributions, by evaluating features such as motivations, types of cited sources or criteria, dates, relations with other claims (e.g. agreement/disagreement). Specifically, historical context regards events and situations that are part of the life-cycle of cultural heritage objects. For instance, "being created by somebody", or "being created at a certain time", are events related to an artefact that are claimed by an agent at a certain time, motivated with usage of primary sources, and recorded in a secondary source (e.g. a cataloguing record). HiCO extends the PROV Ontology with terms for describing aspects of the hermeneutical activity, and reuses existing ontologies, such as CiTO Ontology for linking attributions to related sources."""@en ;
    dc:rights <https://creativecommons.org/licenses/by/4.0/legalcode> ;
    vann:preferredNamespacePrefix "hico" ;
    vann:preferredNamespaceUri "https://w3id.org/hico/" ;
    owl:versionIRI <http://purl.org/emmedi/hico/2020-03-31> ;
    owl:imports skos:, cito:, frbr:, prov:, vann: ;
    owl:versionInfo "2.0" ;
    skos:hasTopConcept hico:InterpretationCriterion, hico:InterpretationType, hico:InterpretationAct;
    foaf:homepage <https://github.com/marilenadaquino/hico> .

hico:InterpretationCriterion a owl:Class, skos:Concept ;
    skos:inScheme <http://purl.org/emmedi/hico/> ;
    skos:topConceptOf <http://purl.org/emmedi/hico/> ;
    rdfs:label "Interpretation Criterion"@en ;
    skos:prefLabel "Interpretation Criterion"@en ;
    rdfs:comment "The criterion or type of source used by an agent to support an interpretation act, such as bibliography, verbal communication, etc. "@en ;
    skos:definition "The criterion or type of source used by an agent to support an interpretation act, such as bibliography, verbal communication, etc. "@en ;
    rdfs:isDefinedBy <http://purl.org/emmedi/hico/> .

hico:InterpretationType a owl:Class, skos:Concept ;
    skos:inScheme <http://purl.org/emmedi/hico/> ;
    skos:topConceptOf <http://purl.org/emmedi/hico/> ;
    rdfs:label "Interpretation Type"@en ;
    skos:prefLabel "Interpretation Type"@en ;
    rdfs:comment "An arbitrary definition of the interpretation act, such as artowork attribution or date attribution."@en ;
    skos:definition "An arbitrary definition of the interpretation act, such as artowork attribution or date attribution."@en ;
    rdfs:isDefinedBy <http://purl.org/emmedi/hico/> .

hico:InterpretationAct a owl:Class, skos:Concept ;
    skos:inScheme <http://purl.org/emmedi/hico/> ;
    skos:topConceptOf <http://purl.org/emmedi/hico/> ;
    rdfs:label "Interpretation Act"@en ;
    skos:prefLabel "Interpretation Act"@en ;
    rdfs:comment "The hermeneutical activity performed by an agent in order to generate new information (e.g. an artwork attribution)."@en ;
    skos:definition "The hermeneutical activity performed by an agent in order to generate new information (e.g. an artwork attribution)."@en ;
    rdfs:isDefinedBy <http://purl.org/emmedi/hico/> ;
    skos:broader prov:Activity ;
    rdfs:subClassOf [ a owl:Restriction ;
            owl:onProperty <http://purl.org/emmedi/hico/hasInterpretationType> ;
            owl:someValuesFrom <http://purl.org/emmedi/hico/InterpretationType> ],
        [ a owl:Restriction ;
            owl:onProperty <http://purl.org/emmedi/hico/isExtractedFrom> ;
            owl:someValuesFrom frbr:Expression ],
        [ a owl:Restriction ;
            owl:onProperty [ owl:inverseOf <http://www.w3.org/TR/prov-o/#wasGeneratedBy> ] ;
            owl:someValuesFrom owl:Thing ],
        [ a owl:Restriction ;
            owl:onProperty <http://purl.org/emmedi/hico/hasInterpretationCriterion> ;
            owl:someValuesFrom <http://purl.org/emmedi/hico/InterpretationCriterion> ],
        prov:Activity .

hico:hasInterpretationCriterion a owl:ObjectProperty, skos:Concept ;
    skos:inScheme <http://purl.org/emmedi/hico/> ;
    rdfs:label "has interpretation criterion"@en ;
    skos:prefLabel "has interpretation criterion"@en ;
    rdfs:comment "A property relating an interpretation act to a criterion or type of source used to support the claim."@en ;
    skos:definition "A property relating an interpretation act to a criterion or type of source used to support the claim."@en ;
    rdfs:domain hico:InterpretationAct ;
    rdfs:isDefinedBy <http://purl.org/emmedi/hico/> ;
    rdfs:range hico:InterpretationCriterion .

hico:hasInterpretationType a owl:ObjectProperty, skos:Concept ;
    skos:inScheme <http://purl.org/emmedi/hico/> ;
    rdfs:label "has interpretation type"@en ;
    skos:prefLabel "has interpretation type"@en ;
    rdfs:comment "A property relating an interpretation act to an individual defining an arbitrary classification of the interpretation."@en ;
    skos:definition "A property relating an interpretation act to an individual defining an arbitrary classification of the interpretation."@en ;
    rdfs:domain hico:InterpretationAct ;
    rdfs:isDefinedBy <http://purl.org/emmedi/hico/> ;
    rdfs:range hico:InterpretationType .

hico:isExtractedFrom a owl:ObjectProperty, skos:Concept ;
    skos:inScheme <http://purl.org/emmedi/hico/> ;
    rdfs:label "is extracted from"@en ;
    skos:prefLabel "is extracted from"@en ;
    rdfs:comment "A property relating an interpretation act to the source where from the claim has been extracted."@en ;
    skos:definition "A property relating an interpretation act to the source where from the claim has been extracted."@en ;
    rdfs:domain hico:InterpretationAct ;
    rdfs:isDefinedBy <http://purl.org/emmedi/hico/> ;
    rdfs:subPropertyOf prov:wasInfluencedBy ;
    skos:broader prov:wasInfluencedBy .

cito:cites a owl:ObjectProperty, skos:Concept ;
    skos:inScheme <http://purl.org/emmedi/hico/> ;
    rdfs:label "cites"@en ;
    skos:prefLabel "cites"@en ;
    rdfs:comment "The citing entity cites the cited entity, either directly and explicitly (as in the reference list of a journal article), indirectly (e.g. by citing a more recent paper by the same group on the same topic), or implicitly (e.g. as in artistic quotations or parodies, or in cases of plagiarism)."@en ;
    skos:definition "The citing entity cites the cited entity, either directly and explicitly (as in the reference list of a journal article), indirectly (e.g. by citing a more recent paper by the same group on the same topic), or implicitly (e.g. as in artistic quotations or parodies, or in cases of plagiarism)."@en ;
    rdfs:isDefinedBy <http://purl.org/spar/cito> .

cito:agreesWith a owl:ObjectProperty, skos:Concept ;
    skos:inScheme <http://purl.org/emmedi/hico/> ;
    rdfs:label "agrees with"@en ;
    skos:prefLabel "agrees with"@en ;
    rdfs:isDefinedBy <http://purl.org/spar/cito> ;
    rdfs:subPropertyOf cito:cites .

cito:citesAsEvidence a owl:ObjectProperty, skos:Concept ;
    skos:inScheme <http://purl.org/emmedi/hico/> ;
    rdfs:label "cites as evidence"@en ;
    skos:prefLabel "cites as evidence"@en ;
    rdfs:isDefinedBy <http://purl.org/spar/cito> ;
    rdfs:subPropertyOf cito:cites .

cito:disagreesWith a owl:ObjectProperty, skos:Concept ;
    skos:inScheme <http://purl.org/emmedi/hico/> ;
    rdfs:label "disagrees with"@en ;
    skos:prefLabel "disagrees with"@en ;
    rdfs:isDefinedBy <http://purl.org/spar/cito> ;
    rdfs:subPropertyOf cito:cites .

cito:refutes a owl:ObjectProperty, skos:Concept ;
    skos:inScheme <http://purl.org/emmedi/hico/> ;
    rdfs:label "refutes"@en ;
    skos:prefLabel "refutes"@en ;
    rdfs:isDefinedBy <http://purl.org/spar/cito> ;
    rdfs:subPropertyOf cito:cites .

prov:startedAtTime a owl:DatatypeProperty, skos:Concept ;
    skos:inScheme <http://purl.org/emmedi/hico/> ;
    rdfs:label "started at time"@en ;
    skos:prefLabel "started at time"@en ;
    rdfs:comment "A property relating an interpretation act to the time that triggered the activity."@en ;
    skos:definition "A property relating an interpretation act to the time that triggered the activity."@en ;
    rdfs:isDefinedBy <http://www.w3.org/ns/prov> ;
    rdfs:range xsd:dateTime .

frbr:Expression a owl:Class, skos:Concept ;
    skos:inScheme <http://purl.org/emmedi/hico/> ;
    rdfs:label "Expression"@en ;
    skos:prefLabel "Expression"@en ;
    rdfs:isDefinedBy <http://purl.org/vocab/frbr/core> .

prov:Activity a owl:Class, skos:Concept ;
    skos:inScheme <http://purl.org/emmedi/hico/> ;
    rdfs:label "Activity"@en ;
    skos:prefLabel "Activity"@en ;
    rdfs:isDefinedBy <http://www.w3.org/ns/prov> .

prov:wasInfluencedBy a owl:ObjectProperty, skos:Concept ;
    skos:inScheme <http://purl.org/emmedi/hico/> ;
    rdfs:label "was influenced by"@en ;
    skos:prefLabel "was influenced by"@en ;
    rdfs:isDefinedBy <http://www.w3.org/ns/prov> .

prov:wasGeneratedBy a owl:ObjectProperty, skos:Concept ;
    skos:inScheme <http://purl.org/emmedi/hico/> ;
    rdfs:label "was generated by"@en ;
    skos:prefLabel "was generated by"@en ;
    rdfs:comment "A property relating statements to an interpretation act."@en ;
    skos:definition  "A property relating statements to an interpretation act."@en ;
    rdfs:isDefinedBy <http://www.w3.org/ns/prov> .

rdfs:domain a rdf:Property ;
	rdfs:isDefinedBy <http://www.w3.org/2000/01/rdf-schema#> ;
	rdfs:label "domain"@en ;
	rdfs:comment "A domain of the subject property."@en ;
    skos:definition  "A domain of the subject property."@en ;
	rdfs:range rdfs:Class ;
	rdfs:domain rdf:Property .

rdfs:range a rdf:Property ;
	rdfs:isDefinedBy <http://www.w3.org/2000/01/rdf-schema#> ;
	rdfs:label "range"@en ;
	rdfs:comment "A range of the subject property."@en ;
    skos:definition "A range of the subject property."@en ;
	rdfs:range rdfs:Class ;
	rdfs:domain rdf:Property .

rdfs:isDefinedBy a rdf:Property ;
	rdfs:isDefinedBy <http://www.w3.org/2000/01/rdf-schema#> ;
	rdfs:label "isDefinedBy"@en ;
	rdfs:comment "The defininition of the subject resource."@en ;
    skos:definition "The defininition of the subject resource."@en ;
	rdfs:range rdfs:Resource ;
	rdfs:domain rdf:Resource .
