@prefix odi: <https://purl.org/ebr/odi#> .
@prefix owl: <http://www.w3.org/2002/07/owl#> .
@prefix rdfs: <http://www.w3.org/2000/01/rdf-schema#> .
@prefix rdf: <http://www.w3.org/1999/02/22-rdf-syntax-ns#> .
@prefix skos: <http://www.w3.org/2004/02/skos/core#> .
@prefix xsd: <http://www.w3.org/2001/XMLSchema#> .
@prefix foaf: <http://xmlns.com/foaf/0.1/> .
@prefix dcat: <http://www.w3.org/ns/dcat#> .
@prefix dct: <http://purl.org/dc/terms/> .  

<https://purl.org/ebr/odi#> a skos:ConceptScheme, owl:Ontology;
    dct:title "Ontologia dei Destini incrociati di Italo Calvino"@it, "Ontology of Italo Calvino's Destini Incrociati"@en;
    rdfs:label "Ontologia dei Destini incrociati di Italo Calvino"@it, "Ontology of Italo Calvino's Destini Incrociati"@en; 
    skos:prefLabel "Ontologia dei Destini incrociati di Italo Calvino"@it, "Ontology of Italo Calvino's Destini Incrociati"@en;
    dct:creator "Enrica Bruno", "Valentina Pasqual", "Francesca Tomasi" ; 
    dct:publisher "/DH.ARC - Digital Humanities Advanced Research Centre"@en, "Dipartimento di Filologia Classica e Italianistica - FICLIT"@it;
    dct:description "ODI (Ontologia dei Destini incrociati di Italo Calvino) is a conceptualization of Italo Calvino's Il castello dei destini incrociati. ODI modules formalise the edition of the work, the description of the cards - both as artefacts and narrative instances - and the semantic links and narrative relations between cards in each story."@en, "ODI (Ontologia dei Destini incrociati di Italo Calvino) è una concettualizzazione di Il castello dei destini incrociati di Italo Calvino. I moduli ODI formalizzano l'edizione dell'opera, la descrizione delle carte - sia come artefatti che come istanze narrative - e i collegamenti semantici e le relazioni narrative tra le carte in ogni racconto."@it ;
    owl:imports skos: ;
    dct:language "English"@en, "Italian"@it ;
    dct:created "2019" ;
    dct:issued "2019-02-01"^^xsd:date ;
    owl:versionInfo "1.0" ;
    skos:hasTopConcept odi:Condition, odi:Dimension, odi:Meaning, odi:Suit, odi:Typology, odi:Person, odi:Place, odi:Storycard, odi:Edition, odi:TarotDeck, odi:DeckCard, odi:Representation ;
    foaf:homepage <https://odi-documentation.github.io/materials/> ;
    dcat:downloadURL <https://odi-documentation.github.io/materials/static/data/odi.owl> .

odi:Person a owl:Class, skos:Concept ;
    skos:inScheme <https://purl.org/ebr/odi#> ;
    skos:topConceptOf <https://purl.org/ebr/odi#> ;
    rdfs:label "Person"@en,
        "Persona"@it ;
    skos:prefLabel "Person"@en,
        "Persona"@it ;
    rdfs:comment "Is a real person related to the book (e.g. the author of the book)."@en,
        "È una persona reale legata al libro (es. l'autore del libro)."@it ;
    skos:definition  "Is a real person related to the book (e.g. the author of the book)."@en,
        "È una persona reale legata al libro (es. l'autore del libro)."@it ;
    rdfs:subClassOf owl:Thing .

odi:Event a owl:Class, skos:Concept ;
    skos:inScheme <https://purl.org/ebr/odi#> ;
    rdfs:label "Evento"@it, "Event"@en ;
    skos:prefLabel "Evento"@it, "Event"@en ;
    rdfs:comment "An event that is carried out by somebody and/or implies something in a story."@en,
        "Un avvenimento che viene eseguito da qualcuno e/o implica degli oggetti in una storia."@it ;
    skos:definition "An event that is carried out by somebody and/or implies something in a story."@en,
        "Un avvenimento che viene eseguito da qualcuno e/o implica degli oggetti in una storia."@it ;
    skos:broader odi:Representation ;
    rdfs:subClassOf odi:Representation .

odi:FictionalPlace a owl:Class, skos:Concept ;
    skos:inScheme <https://purl.org/ebr/odi#> ;
    rdfs:label "Fictional Place"@en,
        "Luogo ideale"@it ;
    skos:prefLabel "Fictional Place"@en,
        "Luogo ideale"@it ;
    rdfs:comment "A place where a character is moving through or arrives at in a story."@en,
        "Un luogo in cui un personaggio si muove o arriva in una storia."@it ;
    skos:broader odi:Representation ;
    rdfs:subClassOf odi:Representation .

odi:Place a owl:Class, skos:Concept ;
    skos:inScheme <https://purl.org/ebr/odi#> ;
    skos:topConceptOf <https://purl.org/ebr/odi#> ;
    rdfs:label "Place"@en,
        "Luogo"@it ;
    skos:prefLabel "Place"@en,
        "Luogo"@it ;
    rdfs:comment "Is a real place related to the book (e.g. the current location of a card)."@en,
        "È un luogo reale legato al libro (es. la collocazione attuale di una carta)."@it ;
    skos:definition "Is a real place related to the book (e.g. the current location of a card)."@en,
        "È un luogo reale legato al libro (es. la collocazione attuale di una carta)."@it ;
    rdfs:subClassOf owl:Thing .

odi:Chapter a owl:Class, skos:Concept ;
    skos:inScheme <https://purl.org/ebr/odi#> ;
    rdfs:label "Chapter"@en,
        "Capitolo"@it ;
    skos:prefLabel "Chapter"@en,
        "Capitolo"@it ;
    rdfs:comment "Is a chapter of the book that contains a story."@en,
        "È un capitolo del libro che contiene una storia."@it ;
    skos:definition "Is a chapter of the book that contains a story."@en,
        "È un capitolo del libro che contiene una storia."@it ;
    skos:broader odi:Edition ;
    skos:narrower odi:Story ; 
    rdfs:subClassOf odi:Edition .

odi:Story a owl:Class, skos:Concept ;
    skos:inScheme <https://purl.org/ebr/odi#> ; ;
    rdfs:label "Story"@en,
        "Storia"@it ;
    skos:prefLabel "Story"@en,
        "Storia"@it ;
    rdfs:comment "A story that makes up the book."@en,
        "Una storia che compone il libro."@it ;
    skos:definition "A story that makes up the book."@en,
        "Una storia che compone il libro."@it ;
    skos:broader odi:Chapter ;
    rdfs:subClassOf odi:Chapter .

odi:Storycard a owl:Class, skos:Concept ;
    skos:inScheme <https://purl.org/ebr/odi#> ;
    skos:topConceptOf <https://purl.org/ebr/odi#> ;
    rdfs:label "Story card"@en,
        "Carta nella storia"@it ;
    skos:prefLabel "Story card"@en,
        "Carta nella storia"@it ;
    rdfs:comment "A card of a story that makes up the book."@en,
        "Una carta di una storia che compone il libro."@it ;
    skos:definition "A card of a story that makes up the book."@en,
        "Una carta di una storia che compone il libro."@it ;
    rdfs:subClassOf owl:Thing .

odi:Edition a owl:Class, skos:Concept ;
    skos:inScheme <https://purl.org/ebr/odi#> ;
    skos:topConceptOf <https://purl.org/ebr/odi#> ;
    rdfs:label "Edition"@en,
        "Edizione"@it ;
    skos:prefLabel "Edition"@en,
        "Edizione"@it ;
    rdfs:comment "It is the edition of the book taken as a reference."@en,
        "È l'edizione del libro presa come riferimento."@it ;
    skos:definition "It is the edition of the book taken as a reference."@en,
        "È l'edizione del libro presa come riferimento."@it ;
    skos:narrower odi:Chapter, odi:PublishingHouse ;
    rdfs:subClassOf owl:Thing .

odi:InanimateObject a owl:Class, skos:Concept ;
    skos:inScheme <https://purl.org/ebr/odi#> ;
    rdfs:label "Inanimate object"@en,
        "Oggetto inanimato"@it ;
    skos:prefLabel "Inanimate object"@en,
        "Oggetto inanimato"@it ;
    rdfs:comment "Every kind of an object in a story."@en,
        "Ogni tipo di oggetto in una storia."@it ;
    skos:definition "Every kind of an object in a story."@en,
        "Ogni tipo di oggetto in una storia."@it ;
    skos:broader odi:Representation ;
    rdfs:subClassOf odi:Representation .

odi:TarotDeck a owl:Class, skos:Concept ;
    skos:inScheme <https://purl.org/ebr/odi#> ;
    skos:topConceptOf <https://purl.org/ebr/odi#> ;
    rdfs:label "Tarot deck"@en,
        "Mazzo di tarocchi"@it ;
    skos:prefLabel "Tarot deck"@en,
        "Mazzo di tarocchi"@it ;
    rdfs:comment "Is a particular type of deck."@en,
        "È un tipo particolare di mazzo."@it ;
    skos:definition  "Is a particular type of deck."@en,
        "È un tipo particolare di mazzo."@it ;
    rdfs:subClassOf owl:Thing .

odi:DeckCard a owl:Class, skos:Concept ;
    skos:inScheme <https://purl.org/ebr/odi#> ;
    skos:topConceptOf <https://purl.org/ebr/odi#> ;
    rdfs:label "Deck card"@en,
        "Carta del mazzo"@it ;
    skos:prefLabel "Deck card"@en,
        "Carta del mazzo"@it ;
    rdfs:comment "Is a card which belongs to the deck."@en,
        "È una carta che appartiene al mazzo."@it ;
    skos:definition "Is a card which belongs to the deck."@en,
        "È una carta che appartiene al mazzo."@it ;
    rdfs:subClassOf owl:Thing .

odi:Representation a owl:Class, skos:Concept ;
    skos:inScheme <https://purl.org/ebr/odi#> ;
    skos:topConceptOf <https://purl.org/ebr/odi#> ;
    rdfs:label "Representation"@en, "Rappresentazione"@it  ;
    skos:prefLabel "Representation"@en, "Rappresentazione"@it  ;
    rdfs:comment 
        "The representation of a card."@en,
        "La rappresentazione di una carta."@it;
    skos:definition         "The representation of a card."@en,
        "La rappresentazione di una carta."@it;
    skos:narrower odi:Event, odi:FictionalPlace, odi:Symbol, odi:Character, odi:InanimateObject ;
    rdfs:subClassOf owl:Thing .

odi:Character a owl:Class, skos:Concept ;
    skos:inScheme <https://purl.org/ebr/odi#> ;
    rdfs:label "Character"@en,
        "Personaggio"@it ;
    skos:prefLabel "Character"@en,
        "Personaggio"@it ;
    rdfs:comment "A character of a story."@en,
        "Un personaggio di una storia."@it ;
    skos:definition "A character of a story."@en,
        "Un personaggio di una storia."@it ;
    skos:broader odi:Representation ;
    rdfs:subClassOf odi:Representation .

odi:Condition a owl:Class, skos:Concept ;
    skos:inScheme <https://purl.org/ebr/odi#> ;
    skos:topConceptOf <https://purl.org/ebr/odi#> ;
    rdfs:label "Condition"@en,
        "Condizione"@it ;
    skos:prefLabel "Condition"@en,
        "Condizione"@it ;
    rdfs:comment "Is the current phisically condition of a card."@en,
        "È lo stato fisico attuale di una carta."@it ;
    skos:definition "Is the current phisically condition of a card."@en,
        "È lo stato fisico attuale di una carta."@it ;
    rdfs:subClassOf owl:Thing .

odi:Dimension a owl:Class, skos:Concept ;
    skos:inScheme <https://purl.org/ebr/odi#> ;
    skos:topConceptOf <https://purl.org/ebr/odi#> ;
    rdfs:label "Dimension"@en,
        "Dimensione"@it ;
    skos:prefLabel "Dimension"@en,
        "Dimensione"@it ;
    rdfs:comment "Is the dimension of the card's iconography in the page of the book."@en,
        "È la dimensione dell'iconografia della carta nella pagina del libro."@it ;
    skos:definition "Is the dimension of the card's iconography in the page of the book."@en,
        "È la dimensione dell'iconografia della carta nella pagina del libro."@it ;
    rdfs:subClassOf owl:Thing .

odi:Meaning a owl:Class, skos:Concept ;
    skos:inScheme <https://purl.org/ebr/odi#> ;
    skos:topConceptOf <https://purl.org/ebr/odi#> ; 
    rdfs:label "Meaning"@en,
        "Significato"@it ;
    skos:prefLabel "Meaning"@en,
        "Significato"@it ;
    rdfs:comment "Is a short meaning of what represent a card in a story."@en,
        "È un breve significato di ciò che rappresenta una carta in una storia."@it ;
    skos:definition "Is a short meaning of what represent a card in a story."@en,
        "È un breve significato di ciò che rappresenta una carta in una storia."@it ;
    rdfs:subClassOf owl:Thing .

odi:PublishingHouse a owl:Class, skos:Concept ;
    skos:inScheme <https://purl.org/ebr/odi#> ;
    rdfs:label "Publishing house"@en,
        "Casa editrice"@it ;
    skos:prefLabel "Publishing house"@en,
        "Casa editrice"@it ;
    rdfs:comment "Is the publishing house of the edition of reference."@en,
        "È la casa editrice dell'edizione di riferimento"@it ;
    skos:definition  "Is the publishing house of the edition of reference."@en,
        "È la casa editrice dell'edizione di riferimento"@it ;
    skos:broader odi:Edition ;
    rdfs:subClassOf odi:Edition .

odi:Suit a owl:Class, skos:Concept ;
    skos:inScheme <https://purl.org/ebr/odi#> ;
    skos:topConceptOf <https://purl.org/ebr/odi#> ;
    rdfs:label "Suit"@en,
        "Seme"@it ;
    skos:prefLabel "Suit"@en,
        "Seme"@it ;
    rdfs:comment "Is the suit of a card."@en,
        "È il seme di una carta."@it ;
    skos:definition "Is the suit of a card."@en,
        "È il seme di una carta."@it ;
    rdfs:subClassOf owl:Thing .

odi:Symbol a owl:Class, skos:Concept ;
    skos:inScheme <https://purl.org/ebr/odi#> ;
    rdfs:label "Symbol"@en,
        "Simbolo"@it ;
    skos:prefLabel "Symbol"@en,
        "Simbolo"@it ;
    rdfs:comment "A symbol or an allegory of something expressed by a card."@en,
        "Un simbolo o un'allegoria di qualcosa espressi da una carta."@it ;
    skos:definition "A symbol or an allegory of something expressed by a card."@en,
        "Un simbolo o un'allegoria di qualcosa espressi da una carta."@it ;
    skos:broader odi:Representation ;
    rdfs:subClassOf odi:Representation .

odi:Typology a owl:Class, skos:Concept ;
    skos:inScheme <https://purl.org/ebr/odi#> ;
    skos:topConceptOf <https://purl.org/ebr/odi#> ;
    rdfs:label "typology"@en,
        "Tipologia"@it ;
    skos:prefLabel "typology"@en,
        "Tipologia"@it ;
    rdfs:comment "Is the typology of the deck and of each card of the deck."@en,
        "È la tipologia del mazzo e di ogni carta del mazzo."@it ;
    skos:definition "Is the typology of the deck and of each card of the deck."@en,
        "È la tipologia del mazzo e di ogni carta del mazzo."@it ;
    rdfs:subClassOf owl:Thing .

odi:arrivesAt a owl:ObjectProperty, skos:Concept ;
    skos:inScheme <https://purl.org/ebr/odi#> ;
    rdfs:label "Arrives at"@en,
        "Arriva a"@it ;
    skos:prefLabel "Arrives at"@en,
        "Arriva a"@it ;
    rdfs:comment "It means that a main character arrives at a place in his story."@en,
        "Significa che un protagonista arriva in un luogo nella sua storia."@it ;
    skos:definition "It means that a main character arrives at a place in his story."@en,
        "Significa che un protagonista arriva in un luogo nella sua storia."@it ;
    rdfs:domain odi:Character ;
    rdfs:range odi:FictionalPlace ;
    rdfs:subPropertyOf owl:topObjectProperty .

odi:bumpsInto a owl:ObjectProperty, skos:Concept ;
    skos:inScheme <https://purl.org/ebr/odi#> ;
    rdfs:label "Bumps into"@en,
        "Si imbatte in"@it ;
    skos:prefLabel "Bumps into"@en,
        "Si imbatte in"@it ;
    rdfs:comment "It means that a main character meets by chance another character during his story."@en,
        "Significa che un protagonista incontra per caso un altro personaggio durante la sua storia."@it ;
    skos:definition "It means that a main character meets by chance another character during his story."@en,
        "Significa che un protagonista incontra per caso un altro personaggio durante la sua storia."@it ;
    rdfs:domain odi:Character ;
    rdfs:range odi:Character ;
    rdfs:subPropertyOf owl:topObjectProperty .

odi:carriedOutby a owl:ObjectProperty, skos:Concept ;
    skos:inScheme <https://purl.org/ebr/odi#> ;
    rdfs:label "Carried out by"@en,
        "È eseguito da"@it ;
    skos:prefLabel "Carried out by"@en,
        "È eseguito da"@it ;
    rdfs:comment "An event is carried out by one or more characters."@en,
        "Un evento viene realizzato da uno o più personaggi."@it ;
    skos:definition  "An event is carried out by one or more characters."@en,
        "Un evento viene realizzato da uno o più personaggi."@it ;
    rdfs:domain odi:Event ;
    rdfs:range odi:Character ;
    rdfs:subPropertyOf owl:topObjectProperty .

odi:carriesRepresentation a owl:ObjectProperty, skos:Concept ;
    skos:inScheme <https://purl.org/ebr/odi#> ;
    rdfs:label "Carries representation"@en,
        "Porta la rappresentazione"@it ;
    skos:prefLabel "Carries representation"@en,
        "Porta la rappresentazione"@it ;
    rdfs:comment "It shows what represent a card in a story."@en,
        "Mostra cosa rappresenta una carta in una storia."@it ;
    skos:definition "It shows what represent a card in a story."@en,
        "Mostra cosa rappresenta una carta in una storia."@it ;
    rdfs:domain odi:Storycard ;
    rdfs:range odi:Representation ;
    rdfs:subPropertyOf owl:topObjectProperty .

odi:changesIn a owl:ObjectProperty, skos:Concept ;
    skos:inScheme <https://purl.org/ebr/odi#> ;
    rdfs:label "Changes in"@en,
        "Cambia in"@it ;
    skos:prefLabel "Changes in"@en,
        "Cambia in"@it ;
    rdfs:comment "This property indicates that a character is represented by two cards representing a different way of being in the same story."@en,
        "Questa proprietà indica che un personaggio è rappresentato da due carte che rappresentano un suo diverso modo di essere nella stessa storia."@it ;
    skos:definition "This property indicates that a character is represented by two cards representing a different way of being in the same story."@en,
        "Questa proprietà indica che un personaggio è rappresentato da due carte che rappresentano un suo diverso modo di essere nella stessa storia."@it ;
    rdfs:domain odi:Character ;
    rdfs:range odi:Character ;
    rdfs:subPropertyOf owl:topObjectProperty .

odi:climbs a owl:ObjectProperty, skos:Concept ;
    skos:inScheme <https://purl.org/ebr/odi#> ;
    rdfs:label "Climbs"@en,
        "Si arrampica"@it ;
    skos:prefLabel "Climbs"@en,
        "Si arrampica"@it ;
    rdfs:comment "This property indicates that a main character climbs a log in his story."@en,
        "Questa proprietà indica che un protagonista si arrampica su un tronco nella sua storia."@it ;
    skos:definition "This property indicates that a main character climbs a log in his story."@en,
        "Questa proprietà indica che un protagonista si arrampica su un tronco nella sua storia."@it ;
    rdfs:range odi:InanimateObject ;
    rdfs:subPropertyOf owl:topObjectProperty .

odi:contains a owl:ObjectProperty, skos:Concept ;
    skos:inScheme <https://purl.org/ebr/odi#> ;
    rdfs:label "Contains"@en,
        "Contiene"@it ;
    skos:prefLabel "Contains"@en,
        "Contiene"@it ;
    rdfs:comment "It connects the tarot deck with its constituent cards."@en,
        "Collega il mazzo di tarocchi con le carte che lo compongono."@it ;
    skos:definition "It connects the tarot deck with its constituent cards."@en,
        "Collega il mazzo di tarocchi con le carte che lo compongono."@it ;
    rdfs:domain odi:TarotDeck ;
    rdfs:range odi:DeckCard ;
    rdfs:subPropertyOf owl:topObjectProperty .

odi:discovers a owl:ObjectPropert, skos:Concept ;
    skos:inScheme <https://purl.org/ebr/odi#> ;
    rdfs:label "Discovers"@en,
        "Scopre"@it ;
    skos:prefLabel "Discovers"@en,
        "Scopre"@it ;
    rdfs:comment "It connects a main character with another character or an event whose true identity or existence is discovered by him during his story."@en,
        "Mette in relazione un protagonista con un altro personaggio o evento la cui vera identità o esistenza viene scoperta da lui nel corso della sua storia."@it ;
    skos:definition "It connects a main character with another character or an event whose true identity or existence is discovered by him during his story."@en,
        "Mette in relazione un protagonista con un altro personaggio o evento la cui vera identità o esistenza viene scoperta da lui nel corso della sua storia."@it ;
    rdfs:domain odi:Character ;
    rdfs:range odi:Character,
        odi:InanimateObject ;
    rdfs:subPropertyOf owl:topObjectProperty .

odi:hasAParticularConditionOf a owl:ObjectProperty, skos:Concept ;
    skos:inScheme <https://purl.org/ebr/odi#> ;
    rdfs:label "Has a particular condition of"@en,
        "Ha una particolare condizione di"@it ;
    skos:prefLabel "Has a particular condition of"@en,
        "Ha una particolare condizione di"@it ;
    rdfs:comment "It shows a particular condition of the main character in his story."@en,
        "Mostra una condizione particolare del protagonista nella sua storia."@it ;
    skos:definition  "It shows a particular condition of the main character in his story."@en,
        "Mostra una condizione particolare del protagonista nella sua storia."@it ;
    rdfs:domain odi:Character ;
    rdfs:range odi:Symbol ;
    rdfs:subPropertyOf owl:topObjectProperty .

odi:hasAuthor a owl:ObjectProperty, skos:Concept ;
    skos:inScheme <https://purl.org/ebr/odi#> ;
    rdfs:label "Has author"@en,
        "Ha autore"@it ;
    skos:prefLabel "Has author"@en,
        "Ha autore"@it ;
    rdfs:comment "This property makes explicit the author of both the tarot deck and a specific card in the tarot deck."@en,
        "Questa proprietà rende esplicito l'autore sia del mazzo di tarocchi sia di una specifica carta del mazzo."@it ;
    skos:definition "This property makes explicit the author of both the tarot deck and a specific card in the tarot deck."@en,
        "Questa proprietà rende esplicito l'autore sia del mazzo di tarocchi sia di una specifica carta del mazzo."@it ;
    rdfs:domain odi:DeckCard,
        odi:Edition,
        odi:TarotDeck ;
    rdfs:range odi:Person ;
    rdfs:subPropertyOf owl:topObjectProperty .

odi:hasCard a owl:ObjectProperty, skos:Concept ;
    skos:inScheme <https://purl.org/ebr/odi#> ;
    rdfs:label "Has card"@en,
        "Ha la carta"@it ;
    skos:prefLabel "Has card"@en,
        "Ha la carta"@it ;
    rdfs:comment "It connects each story with its cards."@en,
        "Collega ogni storia alle sue carte."@it ;
    skos:definition "It connects each story with its cards."@en,
        "Collega ogni storia alle sue carte."@it ;
    rdfs:domain odi:Story ;
    rdfs:range odi:Storycard ;
    rdfs:subPropertyOf owl:topObjectProperty ;
    owl:inverseOf odi:isACardOf .

odi:hasChapter a owl:ObjectProperty, skos:Concept ;
    skos:inScheme <https://purl.org/ebr/odi#> ;
    rdfs:label "Has chapter"@en,
        "Ha capitolo"@it ;
    skos:prefLabel "Has chapter"@en,
        "Ha capitolo"@it ;
    rdfs:comment "This property shows a chapter of the edition of reference."@en,
        "Questa proprietà mostra un capitolo dell'edizione di riferimento."@it ;
    skos:definition "This property shows a chapter of the edition of reference."@en,
        "Questa proprietà mostra un capitolo dell'edizione di riferimento."@it ;
    rdfs:domain odi:Edition ;
    rdfs:range odi:Chapter ;
    rdfs:subPropertyOf owl:topObjectProperty .

odi:hasCurrentLocation a owl:ObjectProperty, skos:Concept ;
    skos:inScheme <https://purl.org/ebr/odi#> ;
    rdfs:label "Has current location"@en,
        "È attualmente conservata"@it ;
    skos:prefLabel "Has current location"@en,
        "È attualmente conservata"@it ;
    rdfs:comment "It indicates the physical location where each card in the deck is stored.",
        "Indica il luogo in cui è attualmente conservata ogni carta del mazzo."@it ;
    skos:definition "It indicates the physical location where each card in the deck is stored.",
        "Indica il luogo in cui è attualmente conservata ogni carta del mazzo."@it ;
    rdfs:domain odi:DeckCard ;
    rdfs:range odi:Place ;
    rdfs:subPropertyOf owl:topObjectProperty .

odi:hasCurrentNumberOfCards a owl:DatatypeProperty, skos:Concept ;
    skos:inScheme <https://purl.org/ebr/odi#> ;
    rdfs:label "Has current number of cards"@en,
        "Ha numero attuale di carte"@it ;
    skos:prefLabel "Has current number of cards"@en,
        "Ha numero attuale di carte"@it ;
    rdfs:comment "It indicates the current number of cards in the tarot deck."@en,
        "Indica il numero attuale di carte del mazzo di tarocchi."@it ;
    skos:definition "It indicates the current number of cards in the tarot deck."@en,
        "Indica il numero attuale di carte del mazzo di tarocchi."@it ;
    rdfs:domain odi:TarotDeck ;
    rdfs:range xsd:integer ;
    rdfs:subPropertyOf owl:topDataProperty .

odi:hasDate a owl:DatatypeProperty, skos:Concept ;
    skos:inScheme <https://purl.org/ebr/odi#> ;
    rdfs:label "Has date"@en,
        "Ha data"@it ;
    skos:prefLabel "Has date"@en,
        "Ha data"@it ;
    rdfs:comment "It indicates the century the tarot deck dates back to."@en,
        "Indica il secolo a cui risale il mazzo di tarocchi."@it ;
    skos:definition  "It indicates the century the tarot deck dates back to."@en,
        "Indica il secolo a cui risale il mazzo di tarocchi."@it ;
    rdfs:domain odi:TarotDeck ;
    rdfs:range xsd:string ;
    rdfs:subPropertyOf owl:topDataProperty .

odi:hasFamilyRelationWith a owl:ObjectProperty, skos:Concept ;
    skos:inScheme <https://purl.org/ebr/odi#> ;
    rdfs:label "Has family relation with"@en,
        "Ha una relazione familiare con"@it ;
    skos:prefLabel "Has family relation with"@en,
        "Ha una relazione familiare con"@it ;
    rdfs:comment "It means that a main character has got a family relation with an another character in his story."@en,
        "Significa che un protagonista ha una relazione familiare con un altro personaggio nella sua storia."@it ;
    skos:definition "It means that a main character has got a family relation with an another character in his story."@en,
        "Significa che un protagonista ha una relazione familiare con un altro personaggio nella sua storia."@it ;
    rdfs:domain odi:Character ;
    rdfs:range odi:Character ;
    rdfs:subPropertyOf owl:topObjectProperty .

odi:hasIconography a owl:ObjectProperty, skos:Concept ;
    skos:inScheme <https://purl.org/ebr/odi#> ;
    rdfs:label "Has iconography"@en,
        "Ha iconografia"@it ;
    skos:prefLabel "Has iconography"@en,
        "Ha iconografia"@it ;
    rdfs:comment "It indicates the dimension of each card's iconography in the page of the book."@en,
        "Indica la dimensione dell'iconografia di ogni carta nella pagina del libro."@it ;
    skos:definition "It indicates the dimension of each card's iconography in the page of the book."@en,
        "Indica la dimensione dell'iconografia di ogni carta nella pagina del libro."@it ;
    rdfs:domain odi:Storycard ;
    rdfs:range odi:Dimension ;
    rdfs:subPropertyOf owl:topObjectProperty .

odi:hasImage a owl:DatatypeProperty, skos:Concept ;
    skos:inScheme <https://purl.org/ebr/odi#> ;
    rdfs:label "Has image"@en,
        "Ha immagine"@it ;
    skos:prefLabel "Has image"@en,
        "Ha immagine"@it ; 
    rdfs:comment "Links to a photo of each card of the tarot deck."@en,
        "Rimanda ad una foto di ogni carta del mazzo di tarocchi."@it ;
    skos:definition "Links to a photo of each card of the tarot deck."@en,
        "Rimanda ad una foto di ogni carta del mazzo di tarocchi."@it ;
    rdfs:domain odi:DeckCard ;
    rdfs:range xsd:anyURI ;
    rdfs:subPropertyOf owl:topDataProperty .

odi:hasIndirectRelationWith a owl:ObjectProperty, skos:Concept ;
    skos:inScheme <https://purl.org/ebr/odi#> ;
    rdfs:label "Has indirect relation with"@en,
        "Ha una relazione indiretta con"@it ;
    skos:prefLabel "Has indirect relation with"@en,
        "Ha una relazione indiretta con"@it ;
    rdfs:comment "This property connects a main character with an element of his story that has no direct link to him, but an indirect link through another card of the story."@en,
        "Questa proprietà collega un protagonista con un elemento della sua storia che non ha un legame diretto con lui, ma un legame indiretto attraverso un'altra carta della storia."@it ;
    skos:definition "This property connects a main character with an element of his story that has no direct link to him, but an indirect link through another card of the story."@en,
        "Questa proprietà collega un protagonista con un elemento della sua storia che non ha un legame diretto con lui, ma un legame indiretto attraverso un'altra carta della storia."@it ;
    rdfs:domain odi:Representation ;
    rdfs:range odi:Representation ;
    rdfs:subPropertyOf owl:topObjectProperty .

odi:hasMeaningOf a owl:ObjectProperty, skos:Concept ;
    skos:inScheme <https://purl.org/ebr/odi#> ;
    rdfs:label "Has meaning of"@en,
        "Ha significato di"@it ;
    skos:prefLabel "Has meaning of"@en,
        "Ha significato di"@it ;
    rdfs:comment "It gives a short description of a card's meaning in a story."@en,
        "Fornisce una breve descrizione del significato di una carta in una storia."@it ;
    skos:definition "It gives a short description of a card's meaning in a story."@en,
        "Fornisce una breve descrizione del significato di una carta in una storia."@it ;
    rdfs:domain odi:Representation ;
    rdfs:range odi:Meaning ;
    rdfs:subPropertyOf owl:topObjectProperty .

odi:hasName a owl:DatatypeProperty, skos:Concept ;
    skos:inScheme <https://purl.org/ebr/odi#> ;
    rdfs:label "Has name"@en,
        "Ha nome"@it ;
    skos:prefLabel "Has name"@en,
        "Ha nome"@it ;
    rdfs:comment "It indicates the specific name of the tarot deck and each of its cards."@en,
        "Indica il nome specifico del mazzo di tarocchi e di ciascuna delle sue carte."@it ;
    skos:definition "It indicates the specific name of the tarot deck and each of its cards."@en,
        "Indica il nome specifico del mazzo di tarocchi e di ciascuna delle sue carte."@it ;
    rdfs:domain odi:TarotDeck ;
    rdfs:range xsd:string ;
    rdfs:subPropertyOf owl:topDataProperty .

odi:hasOriginalNumberOfCards a owl:DatatypeProperty, skos:Concept ;
    skos:inScheme <https://purl.org/ebr/odi#> ;
    rdfs:label "Has original number of cards"@en,
        "Ha numero di carte originariamente"@it ;
    skos:prefLabel "Has original number of cards"@en,
        "Ha numero di carte originariamente"@it ;
    rdfs:comment "It indicates the original number of cards in the tarot deck."@en,
        "Indica il numero originale di carte del mazzo di tarocchi."@it ;
    skos:definition "It indicates the original number of cards in the tarot deck."@en,
        "Indica il numero originale di carte del mazzo di tarocchi."@it ;
    rdfs:domain odi:TarotDeck ;
    rdfs:range xsd:integer ;
    rdfs:subPropertyOf owl:topDataProperty .

odi:hasPositionInTheText a owl:DatatypeProperty, skos:Concept ;
    skos:inScheme <https://purl.org/ebr/odi#> ;
    rdfs:label "Has position in the text"@en,
        "Ha posizione nel testo"@it ;
    skos:prefLabel "Has position in the text"@en,
        "Ha posizione nel testo"@it ;
    rdfs:comment "It indicates the order of appearance of each card in the different stories."@en,
        "Indica l'ordine di apparizione di ogni carta nelle diverse storie."@it ;
    skos:definition "It indicates the order of appearance of each card in the different stories."@en,
        "Indica l'ordine di apparizione di ogni carta nelle diverse storie."@it ;
    rdfs:domain odi:Storycard ;
    rdfs:range xsd:integer ; 
    rdfs:subPropertyOf owl:topDataProperty .

odi:hasPublicationDate a owl:DatatypeProperty, skos:Concept ;
    skos:inScheme <https://purl.org/ebr/odi#> ;
    rdfs:label "Has publication date"@en,
        "Ha data di pubblicazione"@it ;
    skos:prefLabel "Has publication date"@en,
        "Ha data di pubblicazione"@it ;
    rdfs:comment "This property connects the edition of reference with its date of publication."@en,
        "Questa proprietà collega l'edizione di riferimento con la sua data di pubblicazione."@it ;
    skos:definition "This property connects the edition of reference with its date of publication."@en,
        "Questa proprietà collega l'edizione di riferimento con la sua data di pubblicazione."@it ;
    rdfs:domain odi:Edition ;
    rdfs:range xsd:string ;
    rdfs:subPropertyOf owl:topDataProperty .

odi:hasSuit a owl:ObjectProperty, skos:Concept ;
    skos:inScheme <https://purl.org/ebr/odi#> ;
    rdfs:label "Has suit"@en,
        "Ha seme"@it ;
    skos:prefLabel "Has suit"@en,
        "Ha seme"@it ;
    rdfs:comment "It indicates the suit of a card."@en,
        "Indica il seme di una carta."@it ;
    skos:definition "It indicates the suit of a card."@en,
        "Indica il seme di una carta."@it ;
    rdfs:domain odi:DeckCard ;
    rdfs:range odi:Suit ;
    rdfs:subPropertyOf owl:topObjectProperty .

odi:hasTextualReference a owl:DatatypeProperty, skos:Concept ;
    skos:inScheme <https://purl.org/ebr/odi#> ;
    rdfs:label "Has textual reference"@en,
        "Ha riferimento testuale"@it ;
    skos:prefLabel "Has textual reference"@en,
        "Ha riferimento testuale"@it ;
    rdfs:comment "It reports in hooked brackets Calvin's words that give a more accurate description of each card."@en,
        "Riporta tra parentesi uncinate le parole di Calvino che danno una descrizione più accurata di ogni carta."@it ;
    skos:definition "It reports in hooked brackets Calvin's words that give a more accurate description of each card."@en,
        "Riporta tra parentesi uncinate le parole di Calvino che danno una descrizione più accurata di ogni carta."@it ;
    rdfs:domain owl:Thing ;
    rdfs:range xsd:string ;
    rdfs:subPropertyOf owl:topDataProperty .

odi:hasTitle a owl:DatatypeProperty, skos:Concept ;
    skos:inScheme <https://purl.org/ebr/odi#> ;
    rdfs:label "Has title"@en,
        "Ha titolo"@it ;
    skos:prefLabel "Has title"@en,
        "Ha titolo"@it ;
    rdfs:comment "It shows both the title of the reference edition and of a chapter that is also the title of a story."@en,
        "Mostra sia il titolo dell'edizione di riferimento sia di un capitolo che è anche il titolo di una storia."@it ;
    skos:definition "It shows both the title of the reference edition and of a chapter that is also the title of a story."@en,
        "Mostra sia il titolo dell'edizione di riferimento sia di un capitolo che è anche il titolo di una storia."@it ;
    rdfs:domain odi:Chapter,
        odi:Edition,
        odi:Story ;
    rdfs:range xsd:string ;
    rdfs:subPropertyOf owl:topDataProperty .

odi:hasTypology a owl:ObjectProperty, skos:Concept ;
    skos:inScheme <https://purl.org/ebr/odi#> ;
    rdfs:label "Has typology"@en,
        "Ha tipologia"@it ;
    skos:prefLabel "Has typology"@en,
        "Ha tipologia"@it ;
    rdfs:comment "It indicates the typology of the tarot deck and of each of its cards."@en,
        "Indica la tipologia del mazzo di tarocchi e di ciascuna delle sue carte."@it ;
    skos:definition "It indicates the typology of the tarot deck and of each of its cards."@en,
        "Indica la tipologia del mazzo di tarocchi e di ciascuna delle sue carte."@it ;
    rdfs:domain odi:DeckCard,
        odi:TarotDeck ;
    rdfs:range odi:Typology ;
    rdfs:subPropertyOf owl:topObjectProperty .

odi:hasVariantName a owl:DatatypeProperty, skos:Concept ;
    skos:inScheme <https://purl.org/ebr/odi#> ;
    rdfs:label "Has variant name"@en,
        "Ha variante del nome"@it ;
    skos:prefLabel "Has variant name"@en,
        "Ha variante del nome"@it ;
    rdfs:comment "It indicates the variant name of a card in a story."@en,
        "Indica il nome della variante di una carta presente in una storia."@it ;
    skos:definition "It indicates the variant name of a card in a story."@en,
        "Indica il nome della variante di una carta presente in una storia."@it ;
    rdfs:domain odi:Storycard ;
    rdfs:range xsd:string ;
    rdfs:subPropertyOf owl:topDataProperty .

odi:hasVariantNameInTheText a owl:DatatypeProperty, skos:Concept ;
    skos:inScheme <https://purl.org/ebr/odi#> ;
    rdfs:label "has variant name in the text"@en,
        "Ha variante del nome nel testo"@it ;
    skos:prefLabel "has variant name in the text"@en,
        "Ha variante del nome nel testo"@it ;
    rdfs:comment "It indicates which cards have a variant name in the book."@en,
        "Indica quali carte hanno una variante del nome nel libro."@it ;
    skos:definition "It indicates which cards have a variant name in the book."@en,
        "Indica quali carte hanno una variante del nome nel libro."@it ;
    rdfs:domain odi:DeckCard ;
    rdfs:range xsd:string ;
    rdfs:subPropertyOf owl:topDataProperty .

odi:implies a owl:ObjectProperty, skos:Concept ;
    skos:inScheme <https://purl.org/ebr/odi#> ;
    rdfs:label "Implies"@en,
        "Implica"@it ;
    skos:prefLabel "Implies"@en,
        "Implica"@it ;
    rdfs:comment "An event implies one or more objects in a story."@en,
        "Un evento implica uno o più oggetti in una storia."@it ;
    skos:definition  "An event implies one or more objects in a story."@en,
        "Un evento implica uno o più oggetti in una storia."@it ;
    rdfs:domain odi:Event ;
    rdfs:range odi:InanimateObject ;
    rdfs:subPropertyOf owl:topObjectProperty .

odi:includes a owl:ObjectProperty, skos:Concept ;
    skos:inScheme <https://purl.org/ebr/odi#> ;
    rdfs:label "Includes"@en,
        "Include"@it ;
    skos:prefLabel "Includes"@en,
        "Include"@it ;
    rdfs:comment "This property shows a story included in a chapter."@en,
        "Questa proprietà mostra una storia inclusa in un capitolo."@it ;
    skos:definition "This property shows a story included in a chapter."@en,
        "Questa proprietà mostra una storia inclusa in un capitolo."@it ;
    rdfs:domain odi:Chapter ;
    rdfs:range odi:Story ;
    rdfs:subPropertyOf owl:topObjectProperty .

odi:isDefeatedBy a owl:ObjectProperty, skos:Concept ;
    skos:inScheme <https://purl.org/ebr/odi#> ;
    rdfs:label "Is defeated by"@en,
        "È sconfitto da"@it ;
    skos:prefLabel "Is defeated by"@en,
        "È sconfitto da"@it ;
    rdfs:comment "This property indicates that a main character is defeated by another character in his story."@en,
        "Questa proprietà indica che un protagonista viene sconfitto da un altro personaggio nella sua storia."@it ;
    skos:definition "This property indicates that a main character is defeated by another character in his story."@en,
        "Questa proprietà indica che un protagonista viene sconfitto da un altro personaggio nella sua storia."@it ;
    rdfs:domain odi:Character ;
    rdfs:range odi:Character ;
    rdfs:subPropertyOf owl:topObjectProperty .

odi:isHelpedBy a owl:ObjectProperty, skos:Concept ;
    skos:inScheme <https://purl.org/ebr/odi#> ;
    rdfs:label "Is helped by"@en,
        "È aiutato da"@it ;
    skos:prefLabel "Is helped by"@en,
        "È aiutato da"@it ;
    rdfs:comment "This property indicates that a main character is helped by another character in his story."@en,
        "Questa proprietà indica che un protagonista è aiutato da un altro personaggio nella sua storia."@it ;
    skos:definition "This property indicates that a main character is helped by another character in his story."@en,
        "Questa proprietà indica che un protagonista è aiutato da un altro personaggio nella sua storia."@it ;
    rdfs:domain odi:Character ;
    rdfs:range odi:Character ;
    rdfs:subPropertyOf owl:topObjectProperty .

odi:isNumber a owl:DatatypeProperty, skos:Concept ;
    skos:inScheme <https://purl.org/ebr/odi#> ;
    rdfs:label "Is number"@en,
        "È numero"@it ;
    skos:prefLabel  "Is number"@en,
        "È numero"@it ;
    rdfs:comment "It indicates the number representing each number card."@en,
        "Indica il numero che rappresenta ogni \"Numerale\"."@it ;
    skos:definition "It indicates the number representing each number card."@en,
        "Indica il numero che rappresenta ogni \"Numerale\"."@it ;
    rdfs:domain odi:DeckCard ;
    rdfs:range xsd:integer ;
    rdfs:subPropertyOf owl:topDataProperty .

odi:isRelatedWith a owl:ObjectProperty, skos:Concept ;
    skos:inScheme <https://purl.org/ebr/odi#> ;
    rdfs:label "Is related with"@en,
        "È correlata a"@it ;
    skos:prefLabel "Is related with"@en,
        "È correlata a"@it ;
    rdfs:comment "This property connects two cards which have a general relation in a story."@en,
        "Questa proprietà collega due carte che hanno una relazione generale in una storia."@it ;
    skos:definition "This property connects two cards which have a general relation in a story."@en,
        "Questa proprietà collega due carte che hanno una relazione generale in una storia."@it ;    
    rdfs:domain odi:Representation ;
    rdfs:range odi:Representation ;
    rdfs:subPropertyOf owl:topObjectProperty .

odi:isSpecifiedBy a owl:ObjectProperty, skos:Concept ;
    skos:inScheme <https://purl.org/ebr/odi#> ;
    rdfs:label "Is specified by"@en,
        "È specificata da"@it ;
    skos:prefLabel "Is specified by"@en,
        "È specificata da"@it ;
    rdfs:comment "It connects two cards where one specifies the other in a story."@en,
        "Collega due carte in cui una specifica l'altra in una storia."@it ;
    skos:definition "It connects two cards where one specifies the other in a story."@en,
        "Collega due carte in cui una specifica l'altra in una storia."@it ;
    rdfs:domain odi:Representation ;
    rdfs:range odi:Representation ;
    rdfs:subPropertyOf owl:topObjectProperty .

odi:longsFor a owl:ObjectProperty, skos:Concept ;
    skos:inScheme <https://purl.org/ebr/odi#> ;
    rdfs:label "Longs for"@en,
        "Desidera/Brama"@it ;
    skos:prefLabel "Longs for"@en,
        "Desidera/Brama"@it ;
    rdfs:comment "It connects a main character and another character or an object desired by him in his story."@en,
        "Mette in relazione un protagonista e un altro personaggio o un oggetto da lui desiderato nella sua storia."@it ;
    skos:definition "It connects a main character and another character or an object desired by him in his story."@en,
        "Mette in relazione un protagonista e un altro personaggio o un oggetto da lui desiderato nella sua storia."@it ;
    rdfs:domain odi:Character ;
    rdfs:range odi:Character,
        odi:InanimateObject ;
    rdfs:subPropertyOf owl:topObjectProperty .

odi:loses a owl:ObjectProperty, skos:Concept ;
    skos:inScheme <https://purl.org/ebr/odi#> ;
    rdfs:label "Loses"@en,
        "Perde"@it ;
    skos:prefLabel "Loses"@en,
        "Perde"@it ;
    rdfs:comment "It connects a main character and an object which is lost by him in his story."@en,
        "Mette in relazione un protagonista e un oggetto che ha perso nel corso della sua storia."@it ;
    skos:definition "It connects a main character and an object which is lost by him in his story."@en,
        "Mette in relazione un protagonista e un oggetto che ha perso nel corso della sua storia."@it ;
    rdfs:domain odi:Character ;
    rdfs:range odi:InanimateObject ;
    rdfs:subPropertyOf owl:topObjectProperty .

odi:marries a owl:ObjectProperty, skos:Concept ;
    skos:inScheme <https://purl.org/ebr/odi#> ;
    rdfs:label "Marries"@en,
        "Sposa"@it ;
    skos:prefLabel "Marries"@en,
        "Sposa"@it ;
    rdfs:comment "This property indicates a main character who marries a character in his story."@en,
        "Questa proprietà indica un protagonista che sposa un personaggio nella sua storia."@it ;
    skos:definition "This property indicates a main character who marries a character in his story."@en,
        "Questa proprietà indica un protagonista che sposa un personaggio nella sua storia."@it ;
    rdfs:domain odi:Character ;
    rdfs:range odi:Character ;
    rdfs:subPropertyOf owl:topObjectProperty .

odi:movingThrough a owl:ObjectProperty, skos:Concept ;
    skos:inScheme <https://purl.org/ebr/odi#> ;
    rdfs:label "Moving through"@en,
        "Si muove per"@it ;
    skos:prefLabel "Moving through"@en,
        "Si muove per"@it ;
    rdfs:comment "It means that a main character is moving through a place in his story."@en,
        "Significa che un protagonista si muove in un luogo nella sua storia."@it ;
    skos:definition "It means that a main character is moving through a place in his story."@en,
        "Significa che un protagonista si muove in un luogo nella sua storia."@it ;
    rdfs:domain odi:Character ;
    rdfs:range odi:FictionalPlace ;
    rdfs:subPropertyOf owl:topObjectProperty .

odi:placeOfPublication a owl:ObjectProperty, skos:Concept ;
    skos:inScheme <https://purl.org/ebr/odi#> ;
    rdfs:label "Place of publication"@en,
        "Luogo di pubblicazione"@it ;
    skos:prefLabel "Place of publication"@en,
        "Luogo di pubblicazione"@it ;
    rdfs:comment "This property connects the edition of reference with its place of publication."@en,
        "Questa proprietà collega l'edizione di riferimento con il suo luogo di pubblicazione."@it ;
    skos:definition "This property connects the edition of reference with its place of publication."@en,
        "Questa proprietà collega l'edizione di riferimento con il suo luogo di pubblicazione."@it ;
    rdfs:domain odi:Edition ;
    rdfs:range odi:Place ;
    rdfs:subPropertyOf owl:topObjectProperty .

odi:publisher a owl:ObjectProperty, skos:Concept ;
    skos:inScheme <https://purl.org/ebr/odi#> ;
    skos:prefLabel  "Publisher"@en, "Editore"@it;
    rdfs:label  "Publisher"@en, "Editore"@it;
    rdfs:comment 
        "This property connects the edition of reference with its publishing house."@en,
        "Questa proprietà collega l'edizione di riferimento con la sua casa editrice."@it ;
    skos:definition
        "This property connects the edition of reference with its publishing house."@en,
        "Questa proprietà collega l'edizione di riferimento con la sua casa editrice."@it ;
    rdfs:domain odi:Edition ;
    rdfs:range odi:PublishingHouse ;
    rdfs:subPropertyOf owl:topObjectProperty .

odi:receives a owl:ObjectProperty, skos:Concept ;
    skos:inScheme <https://purl.org/ebr/odi#> ;
    rdfs:label "Receives"@en,
        "Riceve"@it ;
    skos:prefLabel "Receives"@en,
        "Riceve"@it ;
    rdfs:comment "It means that a main character receives something during his story."@en,
        "Significa che un protagonista riceve qualcosa durante la sua storia."@it ;
    skos:definition "It means that a main character receives something during his story."@en,
        "Significa che un protagonista riceve qualcosa durante la sua storia."@it ;
    rdfs:domain odi:Character ;
    rdfs:range odi:InanimateObject ;
    rdfs:subPropertyOf owl:topObjectProperty .

odi:represents a owl:ObjectProperty, skos:Concept ;
    skos:inScheme <https://purl.org/ebr/odi#> ;
    rdfs:label "Represents"@en,
        "Rappresenta"@it ;
    skos:prefLabel "Represents"@en,
        "Rappresenta"@it ;
    rdfs:comment "This property shows a character as a person and a fictional place as a place."@en,
        "Mostra cosa rappresenta una carta in una storia."@it ;
    skos:definition "This property shows a character as a person and a fictional place as a place."@en,
        "Mostra cosa rappresenta una carta in una storia."@it ;
    rdfs:domain odi:Character,
        odi:FictionalPlace ;
    rdfs:range odi:Person,
        odi:Place ;
    rdfs:subPropertyOf owl:topObjectProperty .

odi:sameAs a owl:ObjectProperty, skos:Concept ;
    skos:inScheme <https://purl.org/ebr/odi#> ;
    rdfs:label "Same as"@en,
        "È uguale a"@it ;
    skos:prefLabel "Same as"@en,
        "È uguale a"@it ;
    rdfs:comment "This property indicates that two cards represent the same thing."@en,
        "Questa proprietà indica che due carte rappresentano la stessa cosa."@it ;
    skos:definition "This property indicates that two cards represent the same thing."@en,
        "Questa proprietà indica che due carte rappresentano la stessa cosa."@it ;
    rdfs:domain odi:Representation ;
    rdfs:range odi:Representation ;
    rdfs:subPropertyOf owl:topObjectProperty .

odi:sees a owl:ObjectProperty, skos:Concept ;
    skos:inScheme <https://purl.org/ebr/odi#> ;
    rdfs:label "Sees"@en,
        "Vede"@it ;
    skos:prefLabel "Sees"@en,
        "Vede"@it ;
    rdfs:comment "It connects a main character with an event or object seen by him in his story."@en,
        "Mette in relazione un protagonista con un evento o un oggetto visto da lui nella sua storia."@it ;
    skos:definition "It connects a main character with an event or object seen by him in his story."@en,
        "Mette in relazione un protagonista con un evento o un oggetto visto da lui nella sua storia."@it ;
    rdfs:domain odi:Character ;
    rdfs:range odi:Event,
        odi:InanimateObject ;
    rdfs:subPropertyOf owl:topObjectProperty .

odi:speaksTo a owl:ObjectProperty, skos:Concept ;
    skos:inScheme <https://purl.org/ebr/odi#> ;
    rdfs:label "Speaks to"@en,
        "Parla con"@it ;
    skos:prefLabel "Speaks to"@en,
        "Parla con"@it ;
    rdfs:comment "This property shows a main character speaking to another character in a story."@en,
        "Questa proprietà mostra un personaggio principale che parla a un altro personaggio di una storia."@it ;
    skos:definition "This property shows a main character speaking to another character in a story."@en,
        "Questa proprietà mostra un personaggio principale che parla a un altro personaggio di una storia."@it ;
    rdfs:subPropertyOf owl:topObjectProperty .

odi:specifies a owl:ObjectProperty, skos:Concept ;
    skos:inScheme <https://purl.org/ebr/odi#> ;
    rdfs:label "Specifies"@en,
        "Specifica"@it ;
    skos:prefLabel "Specifies"@en,
        "Specifica"@it ;
    rdfs:comment "This property specifies a card of the deck as a card of a story."@en,
        "Questa proprietà specifica una carta del mazzo come carta di una storia."@it ;
    skos:definition "This property specifies a card of the deck as a card of a story."@en,
        "Questa proprietà specifica una carta del mazzo come carta di una storia."@it ;
    rdfs:domain odi:Storycard ;
    rdfs:range odi:DeckCard ;
    rdfs:subPropertyOf owl:topObjectProperty .

odi:trades a owl:ObjectProperty, skos:Concept ;
    skos:inScheme <https://purl.org/ebr/odi#> ;
    rdfs:label "Trades"@en,
        "Baratta"@it ;
    skos:prefLabel "Trades"@en,
        "Baratta"@it ;
    rdfs:comment "This property indicates that a main character trades something in his story."@en,
        "Questa proprietà indica che un protagonista baratta qualcosa nella sua storia."@it ;
    skos:definition  "This property indicates that a main character trades something in his story."@en,
        "Questa proprietà indica che un protagonista baratta qualcosa nella sua storia."@it ;
    rdfs:domain odi:Character ;
    rdfs:range odi:InanimateObject ;
    rdfs:subPropertyOf owl:topObjectProperty .

odi:isACardOf a owl:ObjectProperty, skos:Concept ;
    skos:inScheme <https://purl.org/ebr/odi#> ;
    rdfs:label "Is a card of"@en,
        "È una carta di"@it ;
    skos:prefLabel "Is a card of"@en,
        "È una carta di"@it ;
    rdfs:comment "It connects each card with its story."@en,
        "Collega ogni carta alla sua storia."@it ;
    skos:definition "It connects each card with its story."@en,
        "Collega ogni carta alla sua storia."@it ;
    rdfs:domain odi:Storycard ;
    rdfs:range odi:Story ;
    rdfs:subPropertyOf owl:topObjectProperty .

odi:isContainedIn a owl:ObjectProperty, skos:Concept ;
    skos:inScheme <https://purl.org/ebr/odi#> ;
    rdfs:label "Is contained in"@en,
        "È contenuta in"@it ;
    skos:prefLabel "Is contained in"@en,
        "È contenuta in"@it ;
    rdfs:comment "It connects each card with its tarot deck."@en,
        "Collega ogni carta al relativo mazzo di tarocchi."@it ;
    skos:definition "It connects each card with its tarot deck."@en,
        "Collega ogni carta al relativo mazzo di tarocchi."@it ;
    rdfs:domain odi:DeckCard ;
    rdfs:range odi:TarotDeck ;
    rdfs:subPropertyOf owl:topObjectProperty .

owl:inverseOf a rdf:Property ;
     rdfs:label "inverseOf"@en ;
     rdfs:comment "The property that determines that two given properties are inverse."@en ;
     skos:definition "The property that determines that two given properties are inverse."@en ;
     rdfs:domain owl:ObjectProperty ;
     rdfs:isDefinedBy <http://www.w3.org/2002/07/owl#> ;
     rdfs:range owl:ObjectProperty . 

rdfs:domain a rdf:Property ;
	rdfs:isDefinedBy <http://www.w3.org/2000/01/rdf-schema#> ;
	rdfs:label "domain"@en ;
	rdfs:comment "A domain of the subject property."@en ;
    skos:definition  "A domain of the subject property."@en ;
	rdfs:range rdfs:Class ;
	rdfs:domain rdf:Property .

rdfs:range a rdf:Property ;
	rdfs:isDefinedBy <http://www.w3.org/2000/01/rdf-schema#> ;
	rdfs:label "range"@en ;
	rdfs:comment "A range of the subject property."@en ;
    skos:definition "A range of the subject property."@en ;
	rdfs:range rdfs:Class ;
	rdfs:domain rdf:Property .

rdfs:subClassOf a rdf:Property ;
	rdfs:isDefinedBy <http://www.w3.org/2000/01/rdf-schema#> ;
	rdfs:label "subClassOf" ;
	rdfs:comment "The subject is a subclass of a class." ;
    skos:definition "The subject is a subclass of a class." ;
	rdfs:range rdfs:Class ;
	rdfs:domain rdfs:Class .

dcat:downloadURL a rdf:Property ;
	rdfs:isDefinedBy <http://www.w3.org/TR/vocab-dcat/> ;
	rdfs:label "Download URL"@en ;
	rdfs:comment "The URL of the downloadable file in a given format. E.g. CSV file or RDF file. The format is indicated by the distribution's dct:format and/or dcat:mediaType."@en ;
    skos:definition "The URL of the downloadable file in a given format. E.g. CSV file or RDF file. The format is indicated by the distribution's dct:format and/or dcat:mediaType."@en ;
	rdfs:range rdfs:Resource ;
	rdfs:domain  dcat:Distribution .